code/ecdsa/Hacl.Impl.P.PointAdd.Aux.fst
@@ -11,7 +11,7 @@ open Hacl.Impl.EC.Arithmetics
 open Lib.Buffer
 
 open Hacl.Impl.EC.LowLevel
-open Hacl.Impl.P256.MontgomeryMultiplication
+open Hacl.Impl.EC.MontgomeryMultiplication
 open Spec.P256
 
 open FStar.Tactics 
@@ -19,7 +19,7 @@ open FStar.Tactics.Canon
 
 open FStar.Math.Lemmas
 
-open Hacl.Spec.P.MontgomeryMultiplication
+open Hacl.Spec.MontgomeryMultiplication
 open FStar.Mul
 
 open  Hacl.Spec.P256.Definition
