code/ecdsa/Hacl.Impl.P256.Core.fsti
@@ -12,7 +12,7 @@ open Lib.Buffer
 
 open Hacl.Lemmas.P256
 open Hacl.Spec.P256.Definition
-open Hacl.Spec.P.MontgomeryMultiplication
+open Hacl.Spec.MontgomeryMultiplication
 
 open Spec.P256
 
