code/ecdsa/Hacl.Impl.P256.PointAdd.fst
@@ -21,7 +21,7 @@ open Hacl.Impl.EC.Masking
 open  Hacl.Spec.P256.Definition
 
 
-open Hacl.Spec.P.MontgomeryMultiplication
+open Hacl.Spec.MontgomeryMultiplication
 open FStar.Mul
 
 open Hacl.Impl.P.PointAdd.Aux
