code/ecdsa/Hacl.Impl.P256.PointAdd.fsti
@@ -9,7 +9,7 @@ open Lib.Buffer
 
 open Hacl.Spec.P256.Definition
 open Spec.P256
-open Hacl.Spec.P.MontgomeryMultiplication
+open Hacl.Spec.MontgomeryMultiplication
 
 #set-options "--z3rlimit 100"
 
