code/ecdsa/Hacl.Impl.P256.Signature.Common.fst
@@ -31,8 +31,8 @@ open FStar.Mul
 
 open Hacl.Impl.EC.Arithmetics
 open Hacl.Impl.P256.LowLevel .RawCmp
-open Hacl.Spec.P.MontgomeryMultiplication
-friend Hacl.Spec.P.MontgomeryMultiplication
+open Hacl.Spec.MontgomeryMultiplication
+friend Hacl.Spec.MontgomeryMultiplication
 
 open Hacl.Impl.EC.Intro
 
